<?xml version="1.0"?>
<rdf:RDF xmlns="http://www.example.org/summarization#"
     xml:base="http://www.example.org/summarization"
     xmlns:owl="http://www.w3.org/2002/07/owl#"
     xmlns:rdf="http://www.w3.org/1999/02/22-rdf-syntax-ns#"
     xmlns:xml="http://www.w3.org/XML/1998/namespace"
     xmlns:xsd="http://www.w3.org/2001/XMLSchema#"
     xmlns:rdfs="http://www.w3.org/2000/01/rdf-schema#">
    <owl:Ontology/>
    


    <!-- 
    ///////////////////////////////////////////////////////////////////////////////////////
    //
    // Annotation properties
    //
    ///////////////////////////////////////////////////////////////////////////////////////
     -->

    


    <!-- http://www.example.org/summarization#sourceLink -->

    <owl:AnnotationProperty rdf:about="http://www.example.org/summarization#sourceLink"/>
    


    <!-- 
    ///////////////////////////////////////////////////////////////////////////////////////
    //
    // Object Properties
    //
    ///////////////////////////////////////////////////////////////////////////////////////
     -->

    


    <!-- http://www.example.org/summarization#isAvailableInLanguage -->

    <owl:ObjectProperty rdf:about="http://www.example.org/summarization#isAvailableInLanguage">
        <rdfs:domain rdf:resource="http://www.example.org/summarization#BenchmarkDatasets"/>
        <rdfs:range rdf:resource="http://www.example.org/summarization#Languages"/>
    </owl:ObjectProperty>
    


    <!-- 
    ///////////////////////////////////////////////////////////////////////////////////////
    //
    // Classes
    //
    ///////////////////////////////////////////////////////////////////////////////////////
     -->

    


    <!-- http://www.co-ode.org/ontologies/ont.owl#ReinforcementLearningAbstractive -->

    <owl:Class rdf:about="http://www.co-ode.org/ontologies/ont.owl#ReinforcementLearningAbstractive">
        <rdfs:subClassOf rdf:resource="http://www.example.org/summarization#Extractive"/>
    </owl:Class>
    


    <!-- http://www.example.org/summarization#Abstractive -->

    <owl:Class rdf:about="http://www.example.org/summarization#Abstractive">
        <rdfs:subClassOf rdf:resource="http://www.example.org/summarization#AutomaticTextSummarizationModels"/>
    </owl:Class>
    


    <!-- http://www.example.org/summarization#AttentionBased -->

    <owl:Class rdf:about="http://www.example.org/summarization#AttentionBased">
        <rdfs:subClassOf rdf:resource="http://www.example.org/summarization#Hybrid"/>
    </owl:Class>
    


    <!-- http://www.example.org/summarization#AutomaticTextSummarizationModels -->

    <owl:Class rdf:about="http://www.example.org/summarization#AutomaticTextSummarizationModels"/>
    


    <!-- http://www.example.org/summarization#BenchmarkDatasets -->

    <owl:Class rdf:about="http://www.example.org/summarization#BenchmarkDatasets"/>
    


    <!-- http://www.example.org/summarization#CategorizationAndClassification -->

    <owl:Class rdf:about="http://www.example.org/summarization#CategorizationAndClassification">
        <rdfs:subClassOf rdf:resource="http://www.example.org/summarization#ExtrinsicEvaluationMetrics"/>
    </owl:Class>
    


    <!-- http://www.example.org/summarization#ClaimExtractionBasedEvaluation -->

    <owl:Class rdf:about="http://www.example.org/summarization#ClaimExtractionBasedEvaluation">
        <rdfs:subClassOf rdf:resource="http://www.example.org/summarization#IntrinsicEvaluationMetrics"/>
    </owl:Class>
    


    <!-- http://www.example.org/summarization#English -->

    <owl:Class rdf:about="http://www.example.org/summarization#English">
        <rdfs:subClassOf rdf:resource="http://www.example.org/summarization#Languages"/>
    </owl:Class>
    


    <!-- http://www.example.org/summarization#EvaluationMetrics -->

    <owl:Class rdf:about="http://www.example.org/summarization#EvaluationMetrics"/>
    


    <!-- http://www.example.org/summarization#Extractive -->

    <owl:Class rdf:about="http://www.example.org/summarization#Extractive">
        <rdfs:subClassOf rdf:resource="http://www.example.org/summarization#AutomaticTextSummarizationModels"/>
    </owl:Class>
    


    <!-- http://www.example.org/summarization#ExtrinsicEvaluationMetrics -->

    <owl:Class rdf:about="http://www.example.org/summarization#ExtrinsicEvaluationMetrics">
        <rdfs:subClassOf rdf:resource="http://www.example.org/summarization#EvaluationMetrics"/>
    </owl:Class>
    


    <!-- http://www.example.org/summarization#GraphApproaches -->

    <owl:Class rdf:about="http://www.example.org/summarization#GraphApproaches">
        <rdfs:subClassOf rdf:resource="http://www.example.org/summarization#Extractive"/>
    </owl:Class>
    


    <!-- http://www.example.org/summarization#Hybrid -->

    <owl:Class rdf:about="http://www.example.org/summarization#Hybrid">
        <rdfs:subClassOf rdf:resource="http://www.example.org/summarization#AutomaticTextSummarizationModels"/>
    </owl:Class>
    


    <!-- http://www.example.org/summarization#InformationRetrieval -->

    <owl:Class rdf:about="http://www.example.org/summarization#InformationRetrieval">
        <rdfs:subClassOf rdf:resource="http://www.example.org/summarization#ExtrinsicEvaluationMetrics"/>
    </owl:Class>
    


    <!-- http://www.example.org/summarization#IntrinsicEvaluationMetrics -->

    <owl:Class rdf:about="http://www.example.org/summarization#IntrinsicEvaluationMetrics">
        <rdfs:subClassOf rdf:resource="http://www.example.org/summarization#EvaluationMetrics"/>
    </owl:Class>
    


    <!-- http://www.example.org/summarization#LLMBasedMetrics -->

    <owl:Class rdf:about="http://www.example.org/summarization#LLMBasedMetrics">
        <rdfs:subClassOf rdf:resource="http://www.example.org/summarization#IntrinsicEvaluationMetrics"/>
    </owl:Class>
    


    <!-- http://www.example.org/summarization#Languages -->

    <owl:Class rdf:about="http://www.example.org/summarization#Languages"/>
    


    <!-- http://www.example.org/summarization#LengthBased -->

    <owl:Class rdf:about="http://www.example.org/summarization#LengthBased">
        <rdfs:subClassOf rdf:resource="http://www.example.org/summarization#Extractive"/>
    </owl:Class>
    


    <!-- http://www.example.org/summarization#NLIBasedMetrics -->

    <owl:Class rdf:about="http://www.example.org/summarization#NLIBasedMetrics">
        <rdfs:subClassOf rdf:resource="http://www.example.org/summarization#IntrinsicEvaluationMetrics"/>
    </owl:Class>
    


    <!-- http://www.example.org/summarization#NeuralNetworkApproach -->

    <owl:Class rdf:about="http://www.example.org/summarization#NeuralNetworkApproach">
        <rdfs:subClassOf rdf:resource="http://www.example.org/summarization#Extractive"/>
    </owl:Class>
    


    <!-- http://www.example.org/summarization#Non-English -->

    <owl:Class rdf:about="http://www.example.org/summarization#Non-English">
        <rdfs:subClassOf rdf:resource="http://www.example.org/summarization#Languages"/>
    </owl:Class>
    


    <!-- http://www.example.org/summarization#PointerGeneratorNetworksHybrid -->

    <owl:Class rdf:about="http://www.example.org/summarization#PointerGeneratorNetworksHybrid">
        <rdfs:subClassOf rdf:resource="http://www.example.org/summarization#Hybrid"/>
    </owl:Class>
    


    <!-- http://www.example.org/summarization#QABased -->

    <owl:Class rdf:about="http://www.example.org/summarization#QABased">
        <rdfs:subClassOf rdf:resource="http://www.example.org/summarization#ExtrinsicEvaluationMetrics"/>
    </owl:Class>
    


    <!-- http://www.example.org/summarization#RNNBased -->

    <owl:Class rdf:about="http://www.example.org/summarization#RNNBased">
        <rdfs:subClassOf rdf:resource="http://www.example.org/summarization#Abstractive"/>
    </owl:Class>
    


    <!-- http://www.example.org/summarization#ReinforcementLearning -->

    <owl:Class rdf:about="http://www.example.org/summarization#ReinforcementLearning">
        <rdfs:subClassOf rdf:resource="http://www.example.org/summarization#AutomaticTextSummarizationModels"/>
    </owl:Class>
    


    <!-- http://www.example.org/summarization#ReinforcementLearningAbstractive -->

    <owl:Class rdf:about="http://www.example.org/summarization#ReinforcementLearningAbstractive">
        <rdfs:subClassOf rdf:resource="http://www.example.org/summarization#Abstractive"/>
    </owl:Class>
    


    <!-- http://www.example.org/summarization#ReinforcementLearningHybrid -->

    <owl:Class rdf:about="http://www.example.org/summarization#ReinforcementLearningHybrid">
        <rdfs:subClassOf rdf:resource="http://www.example.org/summarization#Hybrid"/>
    </owl:Class>
    


    <!-- http://www.example.org/summarization#SemanticApproaches -->

    <owl:Class rdf:about="http://www.example.org/summarization#SemanticApproaches">
        <rdfs:subClassOf rdf:resource="http://www.example.org/summarization#Extractive"/>
    </owl:Class>
    


    <!-- http://www.example.org/summarization#SentenceBased -->

    <owl:Class rdf:about="http://www.example.org/summarization#SentenceBased">
        <rdfs:subClassOf rdf:resource="http://www.example.org/summarization#Extractive"/>
    </owl:Class>
    


    <!-- http://www.example.org/summarization#SimilarityBased -->

    <owl:Class rdf:about="http://www.example.org/summarization#SimilarityBased">
        <rdfs:subClassOf rdf:resource="http://www.example.org/summarization#IntrinsicEvaluationMetrics"/>
    </owl:Class>
    


    <!-- http://www.example.org/summarization#SimilarityBasedModels -->

    <owl:Class rdf:about="http://www.example.org/summarization#SimilarityBasedModels">
        <rdfs:subClassOf rdf:resource="http://www.example.org/summarization#Extractive"/>
    </owl:Class>
    


    <!-- http://www.example.org/summarization#TermOverlap -->

    <owl:Class rdf:about="http://www.example.org/summarization#TermOverlap">
        <rdfs:subClassOf rdf:resource="http://www.example.org/summarization#IntrinsicEvaluationMetrics"/>
    </owl:Class>
    


    <!-- http://www.example.org/summarization#TransformerBasedModels -->

    <owl:Class rdf:about="http://www.example.org/summarization#TransformerBasedModels">
        <rdfs:subClassOf rdf:resource="http://www.example.org/summarization#Abstractive"/>
    </owl:Class>
    


    <!-- http://www.example.org/summarization#TransformerBasedModelsHybrid -->

    <owl:Class rdf:about="http://www.example.org/summarization#TransformerBasedModelsHybrid">
        <rdfs:subClassOf rdf:resource="http://www.example.org/summarization#Hybrid"/>
    </owl:Class>
    


    <!-- http://www.example.org/summarization#WordsCountingModels -->

    <owl:Class rdf:about="http://www.example.org/summarization#WordsCountingModels">
        <rdfs:subClassOf rdf:resource="http://www.example.org/summarization#Extractive"/>
    </owl:Class>
    


    <!-- 
    ///////////////////////////////////////////////////////////////////////////////////////
    //
    // Individuals
    //
    ///////////////////////////////////////////////////////////////////////////////////////
     -->

    


    <!-- http://www.co-ode.org/ontologies/ont.owl#BanditSum -->

    <owl:NamedIndividual rdf:about="http://www.co-ode.org/ontologies/ont.owl#BanditSum">
        <rdf:type rdf:resource="http://www.co-ode.org/ontologies/ont.owl#ReinforcementLearningAbstractive"/>
    </owl:NamedIndividual>
    


    <!-- http://www.co-ode.org/ontologies/ont.owl#Seq2Seq -->

    <owl:NamedIndividual rdf:about="http://www.co-ode.org/ontologies/ont.owl#Seq2Seq">
        <rdf:type rdf:resource="http://www.example.org/summarization#RNNBased"/>
    </owl:NamedIndividual>
    


    <!-- http://www.example.org/summarization#ACL -->

    <owl:NamedIndividual rdf:about="http://www.example.org/summarization#ACL">
        <rdf:type rdf:resource="http://www.example.org/summarization#BenchmarkDatasets"/>
    </owl:NamedIndividual>
    


    <!-- http://www.example.org/summarization#ACLAnthology -->

    <owl:NamedIndividual rdf:about="http://www.example.org/summarization#ACLAnthology">
        <rdf:type rdf:resource="http://www.example.org/summarization#BenchmarkDatasets"/>
        <sourceLink>https://aclanthology.org</sourceLink>
    </owl:NamedIndividual>
    


    <!-- http://www.example.org/summarization#ACLDataset -->

    <owl:NamedIndividual rdf:about="http://www.example.org/summarization#ACLDataset">
        <rdf:type rdf:resource="http://www.example.org/summarization#BenchmarkDatasets"/>
        <rdfs:label>Association for Computational Linguistics (ACL) dataset</rdfs:label>
    </owl:NamedIndividual>
    


    <!-- http://www.example.org/summarization#AIAIJDataset -->

    <owl:NamedIndividual rdf:about="http://www.example.org/summarization#AIAIJDataset">
        <rdf:type rdf:resource="http://www.example.org/summarization#BenchmarkDatasets"/>
        <rdfs:label>Artificial intelligence (AI-all) journal dataset</rdfs:label>
    </owl:NamedIndividual>
    


    <!-- http://www.example.org/summarization#AMIMeetingCorpus -->

    <owl:NamedIndividual rdf:about="http://www.example.org/summarization#AMIMeetingCorpus">
        <rdf:type rdf:resource="http://www.example.org/summarization#BenchmarkDatasets"/>
    </owl:NamedIndividual>
    


    <!-- http://www.example.org/summarization#AMN -->

    <owl:NamedIndividual rdf:about="http://www.example.org/summarization#AMN">
        <rdf:type rdf:resource="http://www.example.org/summarization#BenchmarkDatasets"/>
    </owl:NamedIndividual>
    


    <!-- http://www.example.org/summarization#AMRBank -->

    <owl:NamedIndividual rdf:about="http://www.example.org/summarization#AMRBank">
        <rdf:type rdf:resource="http://www.example.org/summarization#BenchmarkDatasets"/>
    </owl:NamedIndividual>
    


    <!-- http://www.example.org/summarization#AQUAINT-2 -->

    <owl:NamedIndividual rdf:about="http://www.example.org/summarization#AQUAINT-2">
        <rdf:type rdf:resource="http://www.example.org/summarization#BenchmarkDatasets"/>
        <isAvailableInLanguage rdf:resource="http://www.example.org/summarization#English"/>
    </owl:NamedIndividual>
    


    <!-- http://www.example.org/summarization#AVIATE -->

    <owl:NamedIndividual rdf:about="http://www.example.org/summarization#AVIATE">
        <rdf:type rdf:resource="http://www.example.org/summarization#BenchmarkDatasets"/>
    </owl:NamedIndividual>
    


    <!-- http://www.example.org/summarization#AbsN -->

    <owl:NamedIndividual rdf:about="http://www.example.org/summarization#AbsN">
        <rdf:type rdf:resource="http://www.example.org/summarization#LengthBased"/>
    </owl:NamedIndividual>
    


    <!-- http://www.example.org/summarization#Absinth -->

    <owl:NamedIndividual rdf:about="http://www.example.org/summarization#Absinth">
        <rdf:type rdf:resource="http://www.example.org/summarization#BenchmarkDatasets"/>
        <isAvailableInLanguage rdf:resource="http://www.example.org/summarization#German"/>
        <sourceLink>https://github.com/mediatechnologycenter/absinth</sourceLink>
    </owl:NamedIndividual>
    


    <!-- http://www.example.org/summarization#AggreFact -->

    <owl:NamedIndividual rdf:about="http://www.example.org/summarization#AggreFact">
        <rdf:type rdf:resource="http://www.example.org/summarization#BenchmarkDatasets"/>
        <sourceLink>https://paperswithcode.com/dataset/aggrefact</sourceLink>
    </owl:NamedIndividual>
    


    <!-- http://www.example.org/summarization#Albanian -->

    <owl:NamedIndividual rdf:about="http://www.example.org/summarization#Albanian">
        <rdf:type rdf:resource="http://www.example.org/summarization#Non-English"/>
    </owl:NamedIndividual>
    


    <!-- http://www.example.org/summarization#AmazonProductReviews -->

    <owl:NamedIndividual rdf:about="http://www.example.org/summarization#AmazonProductReviews">
        <rdf:type rdf:resource="http://www.example.org/summarization#BenchmarkDatasets"/>
        <isAvailableInLanguage rdf:resource="http://www.example.org/summarization#English"/>
        <sourceLink>https://www.amazon.com/product-reviews/</sourceLink>
    </owl:NamedIndividual>
    


    <!-- http://www.example.org/summarization#Amharic -->

    <owl:NamedIndividual rdf:about="http://www.example.org/summarization#Amharic">
        <rdf:type rdf:resource="http://www.example.org/summarization#Non-English"/>
    </owl:NamedIndividual>
    


    <!-- http://www.example.org/summarization#ArXiv -->

    <owl:NamedIndividual rdf:about="http://www.example.org/summarization#ArXiv">
        <rdf:type rdf:resource="http://www.example.org/summarization#BenchmarkDatasets"/>
        <sourceLink>https://arxiv.org/</sourceLink>
    </owl:NamedIndividual>
    


    <!-- http://www.example.org/summarization#Arabic -->

    <owl:NamedIndividual rdf:about="http://www.example.org/summarization#Arabic"/>
    


    <!-- http://www.example.org/summarization#ArabicHeadlineSummary -->

    <owl:NamedIndividual rdf:about="http://www.example.org/summarization#ArabicHeadlineSummary">
        <rdf:type rdf:resource="http://www.example.org/summarization#BenchmarkDatasets"/>
    </owl:NamedIndividual>
    


    <!-- http://www.example.org/summarization#Azerbaijani -->

    <owl:NamedIndividual rdf:about="http://www.example.org/summarization#Azerbaijani">
        <rdf:type rdf:resource="http://www.example.org/summarization#Non-English"/>
    </owl:NamedIndividual>
    


    <!-- http://www.example.org/summarization#BART -->

    <owl:NamedIndividual rdf:about="http://www.example.org/summarization#BART">
        <rdf:type rdf:resource="http://www.example.org/summarization#TransformerBasedModels"/>
        <rdfs:comment>An abstractive summarization model based on Bidirectional and Auto-Regressive Transformers (BART), capable of generating fluent summaries.</rdfs:comment>
    </owl:NamedIndividual>
    


    <!-- http://www.example.org/summarization#BBCArticlesDataset -->

    <owl:NamedIndividual rdf:about="http://www.example.org/summarization#BBCArticlesDataset">
        <rdf:type rdf:resource="http://www.example.org/summarization#BenchmarkDatasets"/>
    </owl:NamedIndividual>
    


    <!-- http://www.example.org/summarization#BBCCNN -->

    <owl:NamedIndividual rdf:about="http://www.example.org/summarization#BBCCNN">
        <rdf:type rdf:resource="http://www.example.org/summarization#BenchmarkDatasets"/>
        <isAvailableInLanguage rdf:resource="http://www.example.org/summarization#English"/>
    </owl:NamedIndividual>
    


    <!-- http://www.example.org/summarization#BC3 -->

    <owl:NamedIndividual rdf:about="http://www.example.org/summarization#BC3">
        <rdf:type rdf:resource="http://www.example.org/summarization#BenchmarkDatasets"/>
        <sourceLink>http://www.cs.ubc.ca/nest/lci/bc3/download.html</sourceLink>
    </owl:NamedIndividual>
    


    <!-- http://www.example.org/summarization#BERT -->

    <owl:NamedIndividual rdf:about="http://www.example.org/summarization#BERT">
        <rdf:type rdf:resource="http://www.example.org/summarization#TransformerBasedModelsHybrid"/>
        <rdfs:comment>An abstractive summarization model based on Bidirectional Encoder Representations from Transformers (BERT), which captures bidirectional contextual information to generate summaries that are more contextually accurate.</rdfs:comment>
    </owl:NamedIndividual>
    


    <!-- http://www.example.org/summarization#BERTExtractiveSum -->

    <owl:NamedIndividual rdf:about="http://www.example.org/summarization#BERTExtractiveSum">
        <rdfs:comment>An extractive summarization model based on BERT embeddings, which selects salient sentences from the input document to form the summary.</rdfs:comment>
    </owl:NamedIndividual>
    


    <!-- http://www.example.org/summarization#BERTScore -->

    <owl:NamedIndividual rdf:about="http://www.example.org/summarization#BERTScore">
        <rdf:type rdf:resource="http://www.example.org/summarization#SimilarityBased"/>
    </owl:NamedIndividual>
    


    <!-- http://www.example.org/summarization#BLEU -->

    <owl:NamedIndividual rdf:about="http://www.example.org/summarization#BLEU">
        <rdf:type rdf:resource="http://www.example.org/summarization#TermOverlap"/>
    </owl:NamedIndividual>
    


    <!-- http://www.example.org/summarization#Bengali -->

    <owl:NamedIndividual rdf:about="http://www.example.org/summarization#Bengali">
        <rdf:type rdf:resource="http://www.example.org/summarization#Non-English"/>
    </owl:NamedIndividual>
    


    <!-- http://www.example.org/summarization#BertSum -->

    <owl:NamedIndividual rdf:about="http://www.example.org/summarization#BertSum">
        <rdfs:comment>An abstractive summarization model that leverages BERT representations to generate concise and coherent summaries.</rdfs:comment>
    </owl:NamedIndividual>
    


    <!-- http://www.example.org/summarization#BertSumExt -->

    <owl:NamedIndividual rdf:about="http://www.example.org/summarization#BertSumExt">
        <rdfs:comment>An extractive summarization model that utilizes BERT embeddings to select salient sentences and generate a concise summary.</rdfs:comment>
    </owl:NamedIndividual>
    


    <!-- http://www.example.org/summarization#Billsum -->

    <owl:NamedIndividual rdf:about="http://www.example.org/summarization#Billsum">
        <rdf:type rdf:resource="http://www.example.org/summarization#BenchmarkDatasets"/>
        <isAvailableInLanguage rdf:resource="http://www.example.org/summarization#English"/>
    </owl:NamedIndividual>
    


    <!-- http://www.example.org/summarization#BookOfHadith -->

    <owl:NamedIndividual rdf:about="http://www.example.org/summarization#BookOfHadith">
        <rdf:type rdf:resource="http://www.example.org/summarization#BenchmarkDatasets"/>
        <isAvailableInLanguage rdf:resource="http://www.example.org/summarization#Indonesian"/>
    </owl:NamedIndividual>
    


    <!-- http://www.example.org/summarization#Bosnian -->

    <owl:NamedIndividual rdf:about="http://www.example.org/summarization#Bosnian">
        <rdf:type rdf:resource="http://www.example.org/summarization#Non-English"/>
    </owl:NamedIndividual>
    


    <!-- http://www.example.org/summarization#BrazilianPortuguese -->

    <owl:NamedIndividual rdf:about="http://www.example.org/summarization#BrazilianPortuguese">
        <rdf:type rdf:resource="http://www.example.org/summarization#Non-English"/>
    </owl:NamedIndividual>
    


    <!-- http://www.example.org/summarization#Bulgarian -->

    <owl:NamedIndividual rdf:about="http://www.example.org/summarization#Bulgarian">
        <rdf:type rdf:resource="http://www.example.org/summarization#Non-English"/>
    </owl:NamedIndividual>
    


    <!-- http://www.example.org/summarization#Burmese -->

    <owl:NamedIndividual rdf:about="http://www.example.org/summarization#Burmese">
        <rdf:type rdf:resource="http://www.example.org/summarization#Non-English"/>
    </owl:NamedIndividual>
    


    <!-- http://www.example.org/summarization#CASTDataset -->

    <owl:NamedIndividual rdf:about="http://www.example.org/summarization#CASTDataset">
        <rdf:type rdf:resource="http://www.example.org/summarization#BenchmarkDatasets"/>
    </owl:NamedIndividual>
    


    <!-- http://www.example.org/summarization#CL-SciSummSharedTask -->

    <owl:NamedIndividual rdf:about="http://www.example.org/summarization#CL-SciSummSharedTask">
        <rdf:type rdf:resource="http://www.example.org/summarization#BenchmarkDatasets"/>
    </owl:NamedIndividual>
    


    <!-- http://www.example.org/summarization#CLSciSummSharedTask -->

    <owl:NamedIndividual rdf:about="http://www.example.org/summarization#CLSciSummSharedTask">
        <rdf:type rdf:resource="http://www.example.org/summarization#BenchmarkDatasets"/>
        <sourceLink>https://github.com/WING-NUS/scisumm-corpus</sourceLink>
    </owl:NamedIndividual>
    


    <!-- http://www.example.org/summarization#CMUMovieSummaryCorpus -->

    <owl:NamedIndividual rdf:about="http://www.example.org/summarization#CMUMovieSummaryCorpus">
        <rdf:type rdf:resource="http://www.example.org/summarization#BenchmarkDatasets"/>
        <sourceLink>http://www.ark.cs.cmu.edu/personas/</sourceLink>
    </owl:NamedIndividual>
    


    <!-- http://www.example.org/summarization#CNN-corpus -->

    <owl:NamedIndividual rdf:about="http://www.example.org/summarization#CNN-corpus">
        <rdf:type rdf:resource="http://www.example.org/summarization#BenchmarkDatasets"/>
    </owl:NamedIndividual>
    


    <!-- http://www.example.org/summarization#CNNDailyMail -->

    <owl:NamedIndividual rdf:about="http://www.example.org/summarization#CNNDailyMail">
        <rdf:type rdf:resource="http://www.example.org/summarization#BenchmarkDatasets"/>
    </owl:NamedIndividual>
    


    <!-- http://www.example.org/summarization#CONCISUSCorpus -->

    <owl:NamedIndividual rdf:about="http://www.example.org/summarization#CONCISUSCorpus">
        <rdf:type rdf:resource="http://www.example.org/summarization#BenchmarkDatasets"/>
        <sourceLink>http://www.taln.upf.edu/pages/concisus/index.html</sourceLink>
    </owl:NamedIndividual>
    


    <!-- http://www.example.org/summarization#CQASumm -->

    <owl:NamedIndividual rdf:about="http://www.example.org/summarization#CQASumm">
        <rdf:type rdf:resource="http://www.example.org/summarization#BenchmarkDatasets"/>
    </owl:NamedIndividual>
    


    <!-- http://www.example.org/summarization#CSTNewsBrazilianCorpus -->

    <owl:NamedIndividual rdf:about="http://www.example.org/summarization#CSTNewsBrazilianCorpus">
        <rdf:type rdf:resource="http://www.example.org/summarization#BenchmarkDatasets"/>
        <isAvailableInLanguage rdf:resource="http://www.example.org/summarization#BrazilianPortuguese"/>
    </owl:NamedIndividual>
    


    <!-- http://www.example.org/summarization#Centroid -->

    <owl:NamedIndividual rdf:about="http://www.example.org/summarization#Centroid">
        <rdfs:comment>An extractive summarization model that represents the document as a centroid of word embeddings and selects sentences closest to this centroid.</rdfs:comment>
    </owl:NamedIndividual>
    


    <!-- http://www.example.org/summarization#CentroidWordEmbed -->

    <owl:NamedIndividual rdf:about="http://www.example.org/summarization#CentroidWordEmbed">
        <rdfs:comment>An extractive summarization model that computes the centroid of word embeddings for each sentence and selects sentences closest to the centroid as the summary.</rdfs:comment>
    </owl:NamedIndividual>
    


    <!-- http://www.example.org/summarization#ChatGPT-CoT -->

    <owl:NamedIndividual rdf:about="http://www.example.org/summarization#ChatGPT-CoT">
        <rdf:type rdf:resource="http://www.example.org/summarization#LLMBasedMetrics"/>
    </owl:NamedIndividual>
    


    <!-- http://www.example.org/summarization#ChatGPT-ZS -->

    <owl:NamedIndividual rdf:about="http://www.example.org/summarization#ChatGPT-ZS">
        <rdf:type rdf:resource="http://www.example.org/summarization#LLMBasedMetrics"/>
    </owl:NamedIndividual>
    


    <!-- http://www.example.org/summarization#Chinese -->

    <owl:NamedIndividual rdf:about="http://www.example.org/summarization#Chinese"/>
    


    <!-- http://www.example.org/summarization#ClusterRank -->

    <owl:NamedIndividual rdf:about="http://www.example.org/summarization#ClusterRank">
        <rdfs:comment>An extractive summarization model that clusters sentences based on their semantic similarity and selects representative sentences from each cluster.</rdfs:comment>
    </owl:NamedIndividual>
    


    <!-- http://www.example.org/summarization#CopyCat -->

    <owl:NamedIndividual rdf:about="http://www.example.org/summarization#CopyCat">
        <rdfs:comment>An abstractive summarization model that employs copy mechanism to handle rare words and named entities, ensuring they are included in the generated summary.</rdfs:comment>
    </owl:NamedIndividual>
    


    <!-- http://www.example.org/summarization#Croatian -->

    <owl:NamedIndividual rdf:about="http://www.example.org/summarization#Croatian">
        <rdf:type rdf:resource="http://www.example.org/summarization#Non-English"/>
    </owl:NamedIndividual>
    


    <!-- http://www.example.org/summarization#Czech -->

    <owl:NamedIndividual rdf:about="http://www.example.org/summarization#Czech">
        <rdf:type rdf:resource="http://www.example.org/summarization#Non-English"/>
    </owl:NamedIndividual>
    


    <!-- http://www.example.org/summarization#DUC -->

    <owl:NamedIndividual rdf:about="http://www.example.org/summarization#DUC">
        <rdf:type rdf:resource="http://www.example.org/summarization#BenchmarkDatasets"/>
        <sourceLink>https://duc.nist.gov</sourceLink>
        <sourceLink>https://www-nlpir.nist.gov/projects/duc/data.html</sourceLink>
    </owl:NamedIndividual>
    


    <!-- http://www.example.org/summarization#DUCTACDataset -->

    <owl:NamedIndividual rdf:about="http://www.example.org/summarization#DUCTACDataset">
        <rdf:type rdf:resource="http://www.example.org/summarization#BenchmarkDatasets"/>
        <rdfs:label>DUC/TAC</rdfs:label>
    </owl:NamedIndividual>
    


    <!-- http://www.example.org/summarization#DeepRLSum -->

    <owl:NamedIndividual rdf:about="http://www.example.org/summarization#DeepRLSum">
        <rdfs:comment>An abstractive summarization model based on Deep Reinforcement Learning (RL) techniques, trained to generate summaries by maximizing summary quality metrics.</rdfs:comment>
    </owl:NamedIndividual>
    


    <!-- http://www.example.org/summarization#DialSummEval -->

    <owl:NamedIndividual rdf:about="http://www.example.org/summarization#DialSummEval">
        <rdf:type rdf:resource="http://www.example.org/summarization#BenchmarkDatasets"/>
    </owl:NamedIndividual>
    


    <!-- http://www.example.org/summarization#DialogSumDataset -->

    <owl:NamedIndividual rdf:about="http://www.example.org/summarization#DialogSumDataset">
        <rdf:type rdf:resource="http://www.example.org/summarization#BenchmarkDatasets"/>
    </owl:NamedIndividual>
    


    <!-- http://www.example.org/summarization#Dutch -->

    <owl:NamedIndividual rdf:about="http://www.example.org/summarization#Dutch">
        <rdf:type rdf:resource="http://www.example.org/summarization#Non-English"/>
    </owl:NamedIndividual>
    


    <!-- http://www.example.org/summarization#EASC -->

    <owl:NamedIndividual rdf:about="http://www.example.org/summarization#EASC">
        <rdf:type rdf:resource="http://www.example.org/summarization#BenchmarkDatasets"/>
        <isAvailableInLanguage rdf:resource="http://www.example.org/summarization#Arabic"/>
    </owl:NamedIndividual>
    


    <!-- http://www.example.org/summarization#EASCEssexArabicSummariesCorpus -->

    <owl:NamedIndividual rdf:about="http://www.example.org/summarization#EASCEssexArabicSummariesCorpus">
        <rdf:type rdf:resource="http://www.example.org/summarization#BenchmarkDatasets"/>
    </owl:NamedIndividual>
    


    <!-- http://www.example.org/summarization#EDT -->

    <owl:NamedIndividual rdf:about="http://www.example.org/summarization#EDT">
        <rdf:type rdf:resource="http://www.example.org/summarization#BenchmarkDatasets"/>
        <rdfs:label>Financial-news based Event-Driven Trading (EDT)</rdfs:label>
    </owl:NamedIndividual>
    


    <!-- http://www.example.org/summarization#ESSEXArabicSummarizationCorpus -->

    <owl:NamedIndividual rdf:about="http://www.example.org/summarization#ESSEXArabicSummarizationCorpus">
        <rdf:type rdf:resource="http://www.example.org/summarization#BenchmarkDatasets"/>
        <sourceLink>http://www.lancaster.ac.uk/staff/elhaj/corpora.htm</sourceLink>
    </owl:NamedIndividual>
    


    <!-- http://www.example.org/summarization#Edmundson -->

    <owl:NamedIndividual rdf:about="http://www.example.org/summarization#Edmundson">
        <rdfs:comment>An extractive summarization model developed by Harold Edmundson, which identifies important sentences based on their occurrence of specific cue words or phrases and their proximity to the beginning of the document, emphasizing the importance of early occurrences.</rdfs:comment>
        <rdfs:comment>An extractive summarization model proposed by Edmundson, which assigns scores to sentences based on various features such as cue words and position.</rdfs:comment>
    </owl:NamedIndividual>
    


    <!-- http://www.example.org/summarization#English -->

    <owl:NamedIndividual rdf:about="http://www.example.org/summarization#English"/>
    


    <!-- http://www.example.org/summarization#FENICE -->

    <owl:NamedIndividual rdf:about="http://www.example.org/summarization#FENICE">
        <rdf:type rdf:resource="http://www.example.org/summarization#ClaimExtractionBasedEvaluation"/>
    </owl:NamedIndividual>
    


    <!-- http://www.example.org/summarization#FastRLE -->

    <owl:NamedIndividual rdf:about="http://www.example.org/summarization#FastRLE">
        <rdf:type rdf:resource="http://www.example.org/summarization#ReinforcementLearning"/>
    </owl:NamedIndividual>
    


    <!-- http://www.example.org/summarization#FinancialNewsBasedEventDrivenTrading -->

    <owl:NamedIndividual rdf:about="http://www.example.org/summarization#FinancialNewsBasedEventDrivenTrading">
        <rdf:type rdf:resource="http://www.example.org/summarization#BenchmarkDatasets"/>
        <sourceLink>https://paperswithcode.com/paper/trade-the-event-corporate-events-detection-for-financial</sourceLink>
    </owl:NamedIndividual>
    


    <!-- http://www.example.org/summarization#French -->

    <owl:NamedIndividual rdf:about="http://www.example.org/summarization#French">
        <rdf:type rdf:resource="http://www.example.org/summarization#Non-English"/>
    </owl:NamedIndividual>
    


    <!-- http://www.example.org/summarization#FrequencySum -->

    <owl:NamedIndividual rdf:about="http://www.example.org/summarization#FrequencySum">
        <rdfs:comment>An extractive summarization model that prioritizes sentences containing important words based on their frequency in the document.</rdfs:comment>
        <rdfs:comment>An extractive summarization model that selects sentences based on their frequency of occurrence in the document, preferring sentences with higher occurrence for inclusion in the summary.</rdfs:comment>
    </owl:NamedIndividual>
    


    <!-- http://www.example.org/summarization#GPT -->

    <owl:NamedIndividual rdf:about="http://www.example.org/summarization#GPT">
        <rdf:type rdf:resource="http://www.example.org/summarization#TransformerBasedModelsHybrid"/>
        <rdfs:comment>An abstractive summarization model based on Generative Pre-trained Transformers (GPT), which employs self-attention mechanisms to generate coherent summaries by predicting words sequentially.</rdfs:comment>
    </owl:NamedIndividual>
    


    <!-- http://www.example.org/summarization#GPTSummarizer -->

    <owl:NamedIndividual rdf:about="http://www.example.org/summarization#GPTSummarizer">
        <rdfs:comment>An abstractive summarization model based on the GPT architecture, capable of generating coherent and contextually relevant summaries.</rdfs:comment>
    </owl:NamedIndividual>
    


    <!-- http://www.example.org/summarization#GatedRecurrentNeuralNetwork -->

    <owl:NamedIndividual rdf:about="http://www.example.org/summarization#GatedRecurrentNeuralNetwork">
        <rdf:type rdf:resource="http://www.example.org/summarization#RNNBased"/>
    </owl:NamedIndividual>
    


    <!-- http://www.example.org/summarization#Gazeta -->

    <owl:NamedIndividual rdf:about="http://www.example.org/summarization#Gazeta">
        <rdf:type rdf:resource="http://www.example.org/summarization#BenchmarkDatasets"/>
        <isAvailableInLanguage rdf:resource="http://www.example.org/summarization#Russian"/>
    </owl:NamedIndividual>
    


    <!-- http://www.example.org/summarization#GensimTextRank -->

    <owl:NamedIndividual rdf:about="http://www.example.org/summarization#GensimTextRank">
        <rdfs:comment>An implementation of TextRank algorithm provided by Gensim library, used for extractive summarization.</rdfs:comment>
    </owl:NamedIndividual>
    


    <!-- http://www.example.org/summarization#German -->

    <owl:NamedIndividual rdf:about="http://www.example.org/summarization#German">
        <rdf:type rdf:resource="http://www.example.org/summarization#Non-English"/>
    </owl:NamedIndividual>
    


    <!-- http://www.example.org/summarization#Gigaword -->

    <owl:NamedIndividual rdf:about="http://www.example.org/summarization#Gigaword">
        <rdf:type rdf:resource="http://www.example.org/summarization#BenchmarkDatasets"/>
    </owl:NamedIndividual>
    


    <!-- http://www.example.org/summarization#Gigaword5 -->

    <owl:NamedIndividual rdf:about="http://www.example.org/summarization#Gigaword5">
        <rdf:type rdf:resource="http://www.example.org/summarization#BenchmarkDatasets"/>
    </owl:NamedIndividual>
    


    <!-- http://www.example.org/summarization#Gujarati -->

    <owl:NamedIndividual rdf:about="http://www.example.org/summarization#Gujarati">
        <rdf:type rdf:resource="http://www.example.org/summarization#Non-English"/>
    </owl:NamedIndividual>
    


    <!-- http://www.example.org/summarization#HASD -->

    <owl:NamedIndividual rdf:about="http://www.example.org/summarization#HASD">
        <rdf:type rdf:resource="http://www.example.org/summarization#BenchmarkDatasets"/>
    </owl:NamedIndividual>
    


    <!-- http://www.example.org/summarization#Hamshahri2Corpus -->

    <owl:NamedIndividual rdf:about="http://www.example.org/summarization#Hamshahri2Corpus">
        <rdf:type rdf:resource="http://www.example.org/summarization#BenchmarkDatasets"/>
        <isAvailableInLanguage rdf:resource="http://www.example.org/summarization#Persian"/>
    </owl:NamedIndividual>
    


    <!-- http://www.example.org/summarization#Hausa -->

    <owl:NamedIndividual rdf:about="http://www.example.org/summarization#Hausa">
        <rdf:type rdf:resource="http://www.example.org/summarization#Non-English"/>
    </owl:NamedIndividual>
    


    <!-- http://www.example.org/summarization#Hebrew -->

    <owl:NamedIndividual rdf:about="http://www.example.org/summarization#Hebrew">
        <rdf:type rdf:resource="http://www.example.org/summarization#Non-English"/>
    </owl:NamedIndividual>
    


    <!-- http://www.example.org/summarization#Hierarchical -->

    <owl:NamedIndividual rdf:about="http://www.example.org/summarization#Hierarchical">
        <rdfs:comment>An extractive summarization model that hierarchically clusters sentences and selects representative sentences from each cluster.</rdfs:comment>
    </owl:NamedIndividual>
    


    <!-- http://www.example.org/summarization#Hindi -->

    <owl:NamedIndividual rdf:about="http://www.example.org/summarization#Hindi"/>
    


    <!-- http://www.example.org/summarization#HindiTextShortSummarizationCorpus -->

    <owl:NamedIndividual rdf:about="http://www.example.org/summarization#HindiTextShortSummarizationCorpus">
        <rdf:type rdf:resource="http://www.example.org/summarization#BenchmarkDatasets"/>
        <isAvailableInLanguage rdf:resource="http://www.example.org/summarization#Hindi"/>
        <sourceLink>https://www.kaggle.com/datasets/disisbig/hindi-text-shortsummarization-corpus</sourceLink>
    </owl:NamedIndividual>
    


    <!-- http://www.example.org/summarization#How2 -->

    <owl:NamedIndividual rdf:about="http://www.example.org/summarization#How2">
        <rdf:type rdf:resource="http://www.example.org/summarization#BenchmarkDatasets"/>
    </owl:NamedIndividual>
    


    <!-- http://www.example.org/summarization#Hungarian -->

    <owl:NamedIndividual rdf:about="http://www.example.org/summarization#Hungarian">
        <rdf:type rdf:resource="http://www.example.org/summarization#Non-English"/>
    </owl:NamedIndividual>
    


    <!-- http://www.example.org/summarization#Igbo -->

    <owl:NamedIndividual rdf:about="http://www.example.org/summarization#Igbo">
        <rdf:type rdf:resource="http://www.example.org/summarization#Non-English"/>
    </owl:NamedIndividual>
    


    <!-- http://www.example.org/summarization#ImageCaptioningCorpus -->

    <owl:NamedIndividual rdf:about="http://www.example.org/summarization#ImageCaptioningCorpus">
        <rdf:type rdf:resource="http://www.example.org/summarization#BenchmarkDatasets"/>
        <sourceLink>http://staffwww.dcs.shef.ac.uk/people/A.Aker/</sourceLink>
    </owl:NamedIndividual>
    


    <!-- http://www.example.org/summarization#Indonesian -->

    <owl:NamedIndividual rdf:about="http://www.example.org/summarization#Indonesian"/>
    


    <!-- http://www.example.org/summarization#Italian -->

    <owl:NamedIndividual rdf:about="http://www.example.org/summarization#Italian">
        <rdf:type rdf:resource="http://www.example.org/summarization#Non-English"/>
    </owl:NamedIndividual>
    


    <!-- http://www.example.org/summarization#JRCMultilingualSummaryEvaluation -->

    <owl:NamedIndividual rdf:about="http://www.example.org/summarization#JRCMultilingualSummaryEvaluation">
        <rdf:type rdf:resource="http://www.example.org/summarization#BenchmarkDatasets"/>
    </owl:NamedIndividual>
    


    <!-- http://www.example.org/summarization#JRCMultilingualSummaryEvaluationData -->

    <owl:NamedIndividual rdf:about="http://www.example.org/summarization#JRCMultilingualSummaryEvaluationData">
        <rdf:type rdf:resource="http://www.example.org/summarization#BenchmarkDatasets"/>
        <sourceLink>https://ec.europa.eu/jrc/en/language-technologies</sourceLink>
        <sourceLink>https://ec.europa.eu/jrc/en/language-technologies/jrc-evaluation-datasets</sourceLink>
    </owl:NamedIndividual>
    


    <!-- http://www.example.org/summarization#Japanese -->

    <owl:NamedIndividual rdf:about="http://www.example.org/summarization#Japanese">
        <rdf:type rdf:resource="http://www.example.org/summarization#Non-English"/>
    </owl:NamedIndividual>
    


    <!-- http://www.example.org/summarization#KALIMAT -->

    <owl:NamedIndividual rdf:about="http://www.example.org/summarization#KALIMAT">
        <rdf:type rdf:resource="http://www.example.org/summarization#BenchmarkDatasets"/>
        <isAvailableInLanguage rdf:resource="http://www.example.org/summarization#Arabic"/>
        <sourceLink>https://sourceforge.net/projects/kalimat/</sourceLink>
    </owl:NamedIndividual>
    


    <!-- http://www.example.org/summarization#KL-Sum -->

    <owl:NamedIndividual rdf:about="http://www.example.org/summarization#KL-Sum">
        <rdfs:comment>An extractive summarization model that employs the KL-Sum algorithm, which selects sentences for inclusion in the summary by maximizing the Kullback-Leibler (KL) divergence between the summary and the original document, ensuring that the summary captures the essential information while minimizing redundancy.</rdfs:comment>
    </owl:NamedIndividual>
    


    <!-- http://www.example.org/summarization#KaggleDatasetHindiMovieReview -->

    <owl:NamedIndividual rdf:about="http://www.example.org/summarization#KaggleDatasetHindiMovieReview">
        <rdf:type rdf:resource="http://www.example.org/summarization#BenchmarkDatasets"/>
        <isAvailableInLanguage rdf:resource="http://www.example.org/summarization#Hindi"/>
    </owl:NamedIndividual>
    


    <!-- http://www.example.org/summarization#KeywordAssociation -->

    <owl:NamedIndividual rdf:about="http://www.example.org/summarization#KeywordAssociation">
        <rdf:type rdf:resource="http://www.example.org/summarization#InformationRetrieval"/>
    </owl:NamedIndividual>
    


    <!-- http://www.example.org/summarization#Kirundi -->

    <owl:NamedIndividual rdf:about="http://www.example.org/summarization#Kirundi">
        <rdf:type rdf:resource="http://www.example.org/summarization#Non-English"/>
    </owl:NamedIndividual>
    


    <!-- http://www.example.org/summarization#Korean -->

    <owl:NamedIndividual rdf:about="http://www.example.org/summarization#Korean">
        <rdf:type rdf:resource="http://www.example.org/summarization#Non-English"/>
    </owl:NamedIndividual>
    


    <!-- http://www.example.org/summarization#KoreanDaumNews -->

    <owl:NamedIndividual rdf:about="http://www.example.org/summarization#KoreanDaumNews">
        <rdf:type rdf:resource="http://www.example.org/summarization#BenchmarkDatasets"/>
    </owl:NamedIndividual>
    


    <!-- http://www.example.org/summarization#Kyrgyz -->

    <owl:NamedIndividual rdf:about="http://www.example.org/summarization#Kyrgyz">
        <rdf:type rdf:resource="http://www.example.org/summarization#Non-English"/>
    </owl:NamedIndividual>
    


    <!-- http://www.example.org/summarization#LCSTS -->

    <owl:NamedIndividual rdf:about="http://www.example.org/summarization#LCSTS">
        <rdf:type rdf:resource="http://www.example.org/summarization#BenchmarkDatasets"/>
        <isAvailableInLanguage rdf:resource="http://www.example.org/summarization#Chinese"/>
        <sourceLink>http://icrc.hitsz.edu.cn/Article/show/139.html</sourceLink>
    </owl:NamedIndividual>
    


    <!-- http://www.example.org/summarization#LEAD -->

    <owl:NamedIndividual rdf:about="http://www.example.org/summarization#LEAD">
        <rdfs:comment>A simple baseline model where the first few sentences of the input text serve as the summary.</rdfs:comment>
    </owl:NamedIndividual>
    


    <!-- http://www.example.org/summarization#LSTM -->

    <owl:NamedIndividual rdf:about="http://www.example.org/summarization#LSTM">
        <rdf:type rdf:resource="http://www.example.org/summarization#RNNBased"/>
        <rdfs:comment>An abstractive summarization model based on Long Short-Term Memory (LSTM) networks, which generate summaries by predicting words sequentially while considering context from the input document.</rdfs:comment>
    </owl:NamedIndividual>
    


    <!-- http://www.example.org/summarization#LSTMTextSum -->

    <owl:NamedIndividual rdf:about="http://www.example.org/summarization#LSTMTextSum">
        <rdfs:comment>An abstractive summarization model that employs Long Short-Term Memory (LSTM) networks to generate summaries by capturing long-range dependencies in text.</rdfs:comment>
    </owl:NamedIndividual>
    


    <!-- http://www.example.org/summarization#LatentDirichletAllocation -->

    <owl:NamedIndividual rdf:about="http://www.example.org/summarization#LatentDirichletAllocation">
        <rdfs:comment>An extractive summarization model based on Latent Dirichlet Allocation (LDA), which identifies topic distributions in the document and selects sentences representing dominant topics for summarization.</rdfs:comment>
    </owl:NamedIndividual>
    


    <!-- http://www.example.org/summarization#LatentSemanticAnalysis -->

    <owl:NamedIndividual rdf:about="http://www.example.org/summarization#LatentSemanticAnalysis">
        <rdf:type rdf:resource="http://www.example.org/summarization#SemanticApproaches"/>
    </owl:NamedIndividual>
    


    <!-- http://www.example.org/summarization#Latvian -->

    <owl:NamedIndividual rdf:about="http://www.example.org/summarization#Latvian">
        <rdf:type rdf:resource="http://www.example.org/summarization#Non-English"/>
    </owl:NamedIndividual>
    


    <!-- http://www.example.org/summarization#Lede3 -->

    <owl:NamedIndividual rdf:about="http://www.example.org/summarization#Lede3">
        <rdf:type rdf:resource="http://www.example.org/summarization#SentenceBased"/>
    </owl:NamedIndividual>
    


    <!-- http://www.example.org/summarization#LexRank -->

    <owl:NamedIndividual rdf:about="http://www.example.org/summarization#LexRank">
        <rdf:type rdf:resource="http://www.example.org/summarization#WordsCountingModels"/>
        <rdfs:comment>An extractive summarization model that applies the LexRank algorithm, which computes sentence importance based on the concept of eigenvector centrality in a graph representation of sentences, considering both the similarity between sentences and their importance scores.</rdfs:comment>
    </owl:NamedIndividual>
    


    <!-- http://www.example.org/summarization#LexicalChainSummarizer -->

    <owl:NamedIndividual rdf:about="http://www.example.org/summarization#LexicalChainSummarizer">
        <rdfs:comment>An extractive summarization model that identifies and leverages lexical chains to select sentences for summarization.</rdfs:comment>
    </owl:NamedIndividual>
    


    <!-- http://www.example.org/summarization#Longformer -->

    <owl:NamedIndividual rdf:about="http://www.example.org/summarization#Longformer">
        <rdfs:comment>An abstractive summarization model based on Longformer architecture, which handles longer document inputs more effectively.</rdfs:comment>
    </owl:NamedIndividual>
    


    <!-- http://www.example.org/summarization#Lsa -->

    <owl:NamedIndividual rdf:about="http://www.example.org/summarization#Lsa">
        <rdfs:comment>An extractive summarization model that uses Latent Semantic Analysis (LSA) to identify important sentences based on semantic similarity.</rdfs:comment>
    </owl:NamedIndividual>
    


    <!-- http://www.example.org/summarization#Luhn -->

    <owl:NamedIndividual rdf:about="http://www.example.org/summarization#Luhn">
        <rdfs:comment>An early extractive summarization model developed by Luhn, which prioritizes sentences containing frequent keywords.</rdfs:comment>
    </owl:NamedIndividual>
    


    <!-- http://www.example.org/summarization#MENLI -->

    <owl:NamedIndividual rdf:about="http://www.example.org/summarization#MENLI">
        <rdf:type rdf:resource="http://www.example.org/summarization#NLIBasedMetrics"/>
    </owl:NamedIndividual>
    


    <!-- http://www.example.org/summarization#METEOR -->

    <owl:NamedIndividual rdf:about="http://www.example.org/summarization#METEOR">
        <rdf:type rdf:resource="http://www.example.org/summarization#TermOverlap"/>
    </owl:NamedIndividual>
    


    <!-- http://www.example.org/summarization#MLSum -->

    <owl:NamedIndividual rdf:about="http://www.example.org/summarization#MLSum">
        <rdf:type rdf:resource="http://www.example.org/summarization#BenchmarkDatasets"/>
        <isAvailableInLanguage rdf:resource="http://www.example.org/summarization#French"/>
        <isAvailableInLanguage rdf:resource="http://www.example.org/summarization#German"/>
        <isAvailableInLanguage rdf:resource="http://www.example.org/summarization#Russian"/>
        <isAvailableInLanguage rdf:resource="http://www.example.org/summarization#Spanish"/>
        <isAvailableInLanguage rdf:resource="http://www.example.org/summarization#Turkish"/>
        <sourceLink>https://huggingface.co/datasets/mlsum</sourceLink>
    </owl:NamedIndividual>
    


    <!-- http://www.example.org/summarization#MMSS -->

    <owl:NamedIndividual rdf:about="http://www.example.org/summarization#MMSS">
        <rdf:type rdf:resource="http://www.example.org/summarization#BenchmarkDatasets"/>
        <isAvailableInLanguage rdf:resource="http://www.example.org/summarization#Arabic"/>
        <isAvailableInLanguage rdf:resource="http://www.example.org/summarization#Bosnian"/>
        <isAvailableInLanguage rdf:resource="http://www.example.org/summarization#Bulgarian"/>
        <isAvailableInLanguage rdf:resource="http://www.example.org/summarization#Czech"/>
        <isAvailableInLanguage rdf:resource="http://www.example.org/summarization#German"/>
    </owl:NamedIndividual>
    


    <!-- http://www.example.org/summarization#MSR-AT -->

    <owl:NamedIndividual rdf:about="http://www.example.org/summarization#MSR-AT">
        <rdf:type rdf:resource="http://www.example.org/summarization#BenchmarkDatasets"/>
    </owl:NamedIndividual>
    


    <!-- http://www.example.org/summarization#Malayalam -->

    <owl:NamedIndividual rdf:about="http://www.example.org/summarization#Malayalam"/>
    


    <!-- http://www.example.org/summarization#MalayalamDocument -->

    <owl:NamedIndividual rdf:about="http://www.example.org/summarization#MalayalamDocument">
        <rdf:type rdf:resource="http://www.example.org/summarization#BenchmarkDatasets"/>
        <isAvailableInLanguage rdf:resource="http://www.example.org/summarization#Malayalam"/>
    </owl:NamedIndividual>
    


    <!-- http://www.example.org/summarization#Marathi -->

    <owl:NamedIndividual rdf:about="http://www.example.org/summarization#Marathi">
        <rdf:type rdf:resource="http://www.example.org/summarization#Non-English"/>
    </owl:NamedIndividual>
    


    <!-- http://www.example.org/summarization#Medline -->

    <owl:NamedIndividual rdf:about="http://www.example.org/summarization#Medline">
        <rdf:type rdf:resource="http://www.example.org/summarization#BenchmarkDatasets"/>
    </owl:NamedIndividual>
    


    <!-- http://www.example.org/summarization#Multi-XScience -->

    <owl:NamedIndividual rdf:about="http://www.example.org/summarization#Multi-XScience">
        <rdf:type rdf:resource="http://www.example.org/summarization#BenchmarkDatasets"/>
    </owl:NamedIndividual>
    


    <!-- http://www.example.org/summarization#MultiLing -->

    <owl:NamedIndividual rdf:about="http://www.example.org/summarization#MultiLing">
        <rdf:type rdf:resource="http://www.example.org/summarization#BenchmarkDatasets"/>
        <sourceLink>http://multiling.iit.demokritos.gr/</sourceLink>
    </owl:NamedIndividual>
    


    <!-- http://www.example.org/summarization#MultiLingPilot -->

    <owl:NamedIndividual rdf:about="http://www.example.org/summarization#MultiLingPilot">
        <rdf:type rdf:resource="http://www.example.org/summarization#BenchmarkDatasets"/>
        <isAvailableInLanguage rdf:resource="http://www.example.org/summarization#English"/>
        <isAvailableInLanguage rdf:resource="http://www.example.org/summarization#French"/>
        <isAvailableInLanguage rdf:resource="http://www.example.org/summarization#Portuguese"/>
        <isAvailableInLanguage rdf:resource="http://www.example.org/summarization#Spanish"/>
    </owl:NamedIndividual>
    


    <!-- http://www.example.org/summarization#MultiXScience -->

    <owl:NamedIndividual rdf:about="http://www.example.org/summarization#MultiXScience">
        <rdf:type rdf:resource="http://www.example.org/summarization#BenchmarkDatasets"/>
        <sourceLink>https://github.com/yaolu/Multi-XScience</sourceLink>
    </owl:NamedIndividual>
    


    <!-- http://www.example.org/summarization#Multinews -->

    <owl:NamedIndividual rdf:about="http://www.example.org/summarization#Multinews">
        <rdf:type rdf:resource="http://www.example.org/summarization#BenchmarkDatasets"/>
    </owl:NamedIndividual>
    


    <!-- http://www.example.org/summarization#NADACorpus -->

    <owl:NamedIndividual rdf:about="http://www.example.org/summarization#NADACorpus">
        <rdf:type rdf:resource="http://www.example.org/summarization#BenchmarkDatasets"/>
    </owl:NamedIndividual>
    


    <!-- http://www.example.org/summarization#NEWSROOM -->

    <owl:NamedIndividual rdf:about="http://www.example.org/summarization#NEWSROOM">
        <rdf:type rdf:resource="http://www.example.org/summarization#BenchmarkDatasets"/>
        <sourceLink>https://lil.nlp.cornell.edu/newsroom/index.html</sourceLink>
    </owl:NamedIndividual>
    


    <!-- http://www.example.org/summarization#NIST -->

    <owl:NamedIndividual rdf:about="http://www.example.org/summarization#NIST">
        <rdf:type rdf:resource="http://www.example.org/summarization#TermOverlap"/>
    </owl:NamedIndividual>
    


    <!-- http://www.example.org/summarization#NLPCC2018 -->

    <owl:NamedIndividual rdf:about="http://www.example.org/summarization#NLPCC2018">
        <rdf:type rdf:resource="http://www.example.org/summarization#BenchmarkDatasets"/>
        <isAvailableInLanguage rdf:resource="http://www.example.org/summarization#Chinese"/>
        <sourceLink>http://tcci.ccf.org.cn/conference/2018/</sourceLink>
    </owl:NamedIndividual>
    


    <!-- http://www.example.org/summarization#NYTDataset -->

    <owl:NamedIndividual rdf:about="http://www.example.org/summarization#NYTDataset">
        <rdf:type rdf:resource="http://www.example.org/summarization#BenchmarkDatasets"/>
        <isAvailableInLanguage rdf:resource="http://www.example.org/summarization#English"/>
    </owl:NamedIndividual>
    


    <!-- http://www.example.org/summarization#Nepali -->

    <owl:NamedIndividual rdf:about="http://www.example.org/summarization#Nepali">
        <rdf:type rdf:resource="http://www.example.org/summarization#Non-English"/>
    </owl:NamedIndividual>
    


    <!-- http://www.example.org/summarization#NeuSum -->

    <owl:NamedIndividual rdf:about="http://www.example.org/summarization#NeuSum">
        <rdf:type rdf:resource="http://www.example.org/summarization#NeuralNetworkApproach"/>
    </owl:NamedIndividual>
    


    <!-- http://www.example.org/summarization#NewYorkTimesAnnotatedCorpus -->

    <owl:NamedIndividual rdf:about="http://www.example.org/summarization#NewYorkTimesAnnotatedCorpus">
        <rdf:type rdf:resource="http://www.example.org/summarization#BenchmarkDatasets"/>
        <sourceLink>https://catalog.ldc.upenn.edu/LDC2008T19</sourceLink>
    </owl:NamedIndividual>
    


    <!-- http://www.example.org/summarization#OAGS -->

    <owl:NamedIndividual rdf:about="http://www.example.org/summarization#OAGS">
        <rdf:type rdf:resource="http://www.example.org/summarization#BenchmarkDatasets"/>
    </owl:NamedIndividual>
    


    <!-- http://www.example.org/summarization#OSAC -->

    <owl:NamedIndividual rdf:about="http://www.example.org/summarization#OSAC">
        <rdf:type rdf:resource="http://www.example.org/summarization#BenchmarkDatasets"/>
    </owl:NamedIndividual>
    


    <!-- http://www.example.org/summarization#Opinosis -->

    <owl:NamedIndividual rdf:about="http://www.example.org/summarization#Opinosis">
        <rdf:type rdf:resource="http://www.example.org/summarization#BenchmarkDatasets"/>
        <isAvailableInLanguage rdf:resource="http://www.example.org/summarization#English"/>
        <sourceLink>http://kavita-ganesan.com/opinosis-opinion-dataset/</sourceLink>
    </owl:NamedIndividual>
    


    <!-- http://www.example.org/summarization#Oromo -->

    <owl:NamedIndividual rdf:about="http://www.example.org/summarization#Oromo">
        <rdf:type rdf:resource="http://www.example.org/summarization#Non-English"/>
    </owl:NamedIndividual>
    


    <!-- http://www.example.org/summarization#PPL -->

    <owl:NamedIndividual rdf:about="http://www.example.org/summarization#PPL">
        <rdf:type rdf:resource="http://www.example.org/summarization#TermOverlap"/>
    </owl:NamedIndividual>
    


    <!-- http://www.example.org/summarization#PageRank -->

    <owl:NamedIndividual rdf:about="http://www.example.org/summarization#PageRank">
        <rdf:type rdf:resource="http://www.example.org/summarization#GraphApproaches"/>
        <rdfs:comment>An extractive summarization model that applies PageRank algorithm to identify key sentences based on their connectivity in the document.</rdfs:comment>
    </owl:NamedIndividual>
    


    <!-- http://www.example.org/summarization#Pashto -->

    <owl:NamedIndividual rdf:about="http://www.example.org/summarization#Pashto">
        <rdf:type rdf:resource="http://www.example.org/summarization#Non-English"/>
    </owl:NamedIndividual>
    


    <!-- http://www.example.org/summarization#PasokhCorpus -->

    <owl:NamedIndividual rdf:about="http://www.example.org/summarization#PasokhCorpus">
        <rdf:type rdf:resource="http://www.example.org/summarization#BenchmarkDatasets"/>
        <isAvailableInLanguage rdf:resource="http://www.example.org/summarization#Persian"/>
    </owl:NamedIndividual>
    


    <!-- http://www.example.org/summarization#Pegasus -->

    <owl:NamedIndividual rdf:about="http://www.example.org/summarization#Pegasus">
        <rdfs:comment>An abstractive summarization model based on Pre-trained Encoder-decoder with Masked Language Model objectives for Generation and Summarization (PEGASUS).</rdfs:comment>
    </owl:NamedIndividual>
    


    <!-- http://www.example.org/summarization#Persian -->

    <owl:NamedIndividual rdf:about="http://www.example.org/summarization#Persian">
        <rdf:type rdf:resource="http://www.example.org/summarization#Non-English"/>
    </owl:NamedIndividual>
    


    <!-- http://www.example.org/summarization#Pidgina -->

    <owl:NamedIndividual rdf:about="http://www.example.org/summarization#Pidgina">
        <rdf:type rdf:resource="http://www.example.org/summarization#Non-English"/>
    </owl:NamedIndividual>
    


    <!-- http://www.example.org/summarization#PointerGeneratorNetwork -->

    <owl:NamedIndividual rdf:about="http://www.example.org/summarization#PointerGeneratorNetwork">
        <rdfs:comment>An abstractive summarization model that combines extractive and abstractive approaches using a Pointer-Generator Network, allowing it to copy words from the input document and generate novel phrases for the summary.</rdfs:comment>
        <rdfs:comment>An abstractive summarization model that integrates copying mechanism and generation to handle out-of-vocabulary words, based on Pointer-Generator Networks.</rdfs:comment>
    </owl:NamedIndividual>
    


    <!-- http://www.example.org/summarization#PointerGeneratorNetworks -->

    <owl:NamedIndividual rdf:about="http://www.example.org/summarization#PointerGeneratorNetworks">
        <rdf:type rdf:resource="http://www.example.org/summarization#RNNBased"/>
    </owl:NamedIndividual>
    


    <!-- http://www.example.org/summarization#PointerGeneratorNetworksHybrid -->

    <owl:NamedIndividual rdf:about="http://www.example.org/summarization#PointerGeneratorNetworksHybrid">
        <rdf:type rdf:resource="http://www.example.org/summarization#PointerGeneratorNetworksHybrid"/>
    </owl:NamedIndividual>
    


    <!-- http://www.example.org/summarization#Polish -->

    <owl:NamedIndividual rdf:about="http://www.example.org/summarization#Polish">
        <rdf:type rdf:resource="http://www.example.org/summarization#Non-English"/>
    </owl:NamedIndividual>
    


    <!-- http://www.example.org/summarization#PolstatSTIS -->

    <owl:NamedIndividual rdf:about="http://www.example.org/summarization#PolstatSTIS">
        <rdf:type rdf:resource="http://www.example.org/summarization#BenchmarkDatasets"/>
        <isAvailableInLanguage rdf:resource="http://www.example.org/summarization#Indonesian"/>
    </owl:NamedIndividual>
    


    <!-- http://www.example.org/summarization#Portuguese -->

    <owl:NamedIndividual rdf:about="http://www.example.org/summarization#Portuguese">
        <rdf:type rdf:resource="http://www.example.org/summarization#Non-English"/>
    </owl:NamedIndividual>
    


    <!-- http://www.example.org/summarization#ProphetNet -->

    <owl:NamedIndividual rdf:about="http://www.example.org/summarization#ProphetNet">
        <rdfs:comment>An abstractive summarization model that utilizes masked self-attention mechanism and cross-attention to generate summaries, based on ProphetNet architecture.</rdfs:comment>
    </owl:NamedIndividual>
    


    <!-- http://www.example.org/summarization#PubMedQA -->

    <owl:NamedIndividual rdf:about="http://www.example.org/summarization#PubMedQA">
        <rdf:type rdf:resource="http://www.example.org/summarization#BenchmarkDatasets"/>
        <sourceLink>https://pubmedqa.github.io/</sourceLink>
    </owl:NamedIndividual>
    


    <!-- http://www.example.org/summarization#Punjabi -->

    <owl:NamedIndividual rdf:about="http://www.example.org/summarization#Punjabi">
        <rdf:type rdf:resource="http://www.example.org/summarization#Non-English"/>
    </owl:NamedIndividual>
    


    <!-- http://www.example.org/summarization#QMSum -->

    <owl:NamedIndividual rdf:about="http://www.example.org/summarization#QMSum">
        <rdf:type rdf:resource="http://www.example.org/summarization#BenchmarkDatasets"/>
        <sourceLink>https://github.com/Yale-LILY/QMSum</sourceLink>
    </owl:NamedIndividual>
    


    <!-- http://www.example.org/summarization#QuestEval -->

    <owl:NamedIndividual rdf:about="http://www.example.org/summarization#QuestEval">
        <rdf:type rdf:resource="http://www.example.org/summarization#QABased"/>
    </owl:NamedIndividual>
    


    <!-- http://www.example.org/summarization#ROUGE -->

    <owl:NamedIndividual rdf:about="http://www.example.org/summarization#ROUGE">
        <rdf:type rdf:resource="http://www.example.org/summarization#TermOverlap"/>
    </owl:NamedIndividual>
    


    <!-- http://www.example.org/summarization#RTAnews -->

    <owl:NamedIndividual rdf:about="http://www.example.org/summarization#RTAnews">
        <rdf:type rdf:resource="http://www.example.org/summarization#BenchmarkDatasets"/>
        <sourceLink>https://data.mendeley.com/datasets/322pzsdxwy/1</sourceLink>
    </owl:NamedIndividual>
    


    <!-- http://www.example.org/summarization#RandomSum -->

    <owl:NamedIndividual rdf:about="http://www.example.org/summarization#RandomSum">
        <rdfs:comment>An extractive summarization model that randomly selects sentences from the input document to form the summary.</rdfs:comment>
    </owl:NamedIndividual>
    


    <!-- http://www.example.org/summarization#Rechtspraak -->

    <owl:NamedIndividual rdf:about="http://www.example.org/summarization#Rechtspraak">
        <rdf:type rdf:resource="http://www.example.org/summarization#BenchmarkDatasets"/>
        <isAvailableInLanguage rdf:resource="http://www.example.org/summarization#Dutch"/>
        <sourceLink>https://data.overheid.nl/dataset/uitspraken-rechtspraak-nl</sourceLink>
    </owl:NamedIndividual>
    


    <!-- http://www.example.org/summarization#RecurrentNeuralNetworks -->

    <owl:NamedIndividual rdf:about="http://www.example.org/summarization#RecurrentNeuralNetworks">
        <rdf:type rdf:resource="http://www.example.org/summarization#NeuralNetworkApproach"/>
    </owl:NamedIndividual>
    


    <!-- http://www.example.org/summarization#RedditTIFU -->

    <owl:NamedIndividual rdf:about="http://www.example.org/summarization#RedditTIFU">
        <rdf:type rdf:resource="http://www.example.org/summarization#BenchmarkDatasets"/>
        <isAvailableInLanguage rdf:resource="http://www.example.org/summarization#English"/>
    </owl:NamedIndividual>
    


    <!-- http://www.example.org/summarization#RestrictedBoltzmannMachine -->

    <owl:NamedIndividual rdf:about="http://www.example.org/summarization#RestrictedBoltzmannMachine">
        <rdf:type rdf:resource="http://www.example.org/summarization#NeuralNetworkApproach"/>
    </owl:NamedIndividual>
    


    <!-- http://www.example.org/summarization#RetrieveAndSummarize -->

    <owl:NamedIndividual rdf:about="http://www.example.org/summarization#RetrieveAndSummarize">
        <rdfs:comment>An extractive summarization model that first retrieves relevant passages from a large corpus and then generates a summary based on the retrieved passages.</rdfs:comment>
    </owl:NamedIndividual>
    


    <!-- http://www.example.org/summarization#Russian -->

    <owl:NamedIndividual rdf:about="http://www.example.org/summarization#Russian">
        <rdf:type rdf:resource="http://www.example.org/summarization#Non-English"/>
    </owl:NamedIndividual>
    


    <!-- http://www.example.org/summarization#SAMSum -->

    <owl:NamedIndividual rdf:about="http://www.example.org/summarization#SAMSum">
        <rdf:type rdf:resource="http://www.example.org/summarization#BenchmarkDatasets"/>
        <sourceLink>https://huggingface.co/datasets/samsum</sourceLink>
    </owl:NamedIndividual>
    


    <!-- http://www.example.org/summarization#SANAD -->

    <owl:NamedIndividual rdf:about="http://www.example.org/summarization#SANAD">
        <rdf:type rdf:resource="http://www.example.org/summarization#BenchmarkDatasets"/>
        <sourceLink>https://www.kaggle.com/datasets/haithemhermessi/sanad-dataset</sourceLink>
    </owl:NamedIndividual>
    


    <!-- http://www.example.org/summarization#SIFRank -->

    <owl:NamedIndividual rdf:about="http://www.example.org/summarization#SIFRank">
        <rdfs:comment>An extractive summarization model that utilizes Smooth Inverse Frequency (SIF) embeddings and PageRank algorithm to identify important sentences.</rdfs:comment>
    </owl:NamedIndividual>
    


    <!-- http://www.example.org/summarization#SIGIR2018Corpus -->

    <owl:NamedIndividual rdf:about="http://www.example.org/summarization#SIGIR2018Corpus">
        <rdf:type rdf:resource="http://www.example.org/summarization#BenchmarkDatasets"/>
    </owl:NamedIndividual>
    


    <!-- http://www.example.org/summarization#SUMPUBMED -->

    <owl:NamedIndividual rdf:about="http://www.example.org/summarization#SUMPUBMED">
        <rdf:type rdf:resource="http://www.example.org/summarization#BenchmarkDatasets"/>
        <isAvailableInLanguage rdf:resource="http://www.example.org/summarization#English"/>
    </owl:NamedIndividual>
    


    <!-- http://www.example.org/summarization#ScisummNet -->

    <owl:NamedIndividual rdf:about="http://www.example.org/summarization#ScisummNet">
        <rdf:type rdf:resource="http://www.example.org/summarization#BenchmarkDatasets"/>
    </owl:NamedIndividual>
    


    <!-- http://www.example.org/summarization#Scopus -->

    <owl:NamedIndividual rdf:about="http://www.example.org/summarization#Scopus">
        <rdf:type rdf:resource="http://www.example.org/summarization#BenchmarkDatasets"/>
        <isAvailableInLanguage rdf:resource="http://www.example.org/summarization#English"/>
        <sourceLink>https://www.scopus.com/</sourceLink>
    </owl:NamedIndividual>
    


    <!-- http://www.example.org/summarization#ScottishGaelic -->

    <owl:NamedIndividual rdf:about="http://www.example.org/summarization#ScottishGaelic">
        <rdf:type rdf:resource="http://www.example.org/summarization#Non-English"/>
    </owl:NamedIndividual>
    


    <!-- http://www.example.org/summarization#SelfMadeDataset -->

    <owl:NamedIndividual rdf:about="http://www.example.org/summarization#SelfMadeDataset">
        <rdf:type rdf:resource="http://www.example.org/summarization#BenchmarkDatasets"/>
        <isAvailableInLanguage rdf:resource="http://www.example.org/summarization#English"/>
        <rdfs:label>Self-made dataset</rdfs:label>
    </owl:NamedIndividual>
    


    <!-- http://www.example.org/summarization#SemanticRoleLabelling -->

    <owl:NamedIndividual rdf:about="http://www.example.org/summarization#SemanticRoleLabelling">
        <rdf:type rdf:resource="http://www.example.org/summarization#SemanticApproaches"/>
    </owl:NamedIndividual>
    


    <!-- http://www.example.org/summarization#SentenceBERT -->

    <owl:NamedIndividual rdf:about="http://www.example.org/summarization#SentenceBERT">
        <rdf:type rdf:resource="http://www.example.org/summarization#SentenceBased"/>
    </owl:NamedIndividual>
    


    <!-- http://www.example.org/summarization#Seq2Seq -->

    <owl:NamedIndividual rdf:about="http://www.example.org/summarization#Seq2Seq">
        <rdfs:comment>An abstractive summarization model based on Sequence-to-Sequence (Seq2Seq) architecture, consisting of encoder-decoder framework for generating summaries.</rdfs:comment>
    </owl:NamedIndividual>
    


    <!-- http://www.example.org/summarization#Serbian -->

    <owl:NamedIndividual rdf:about="http://www.example.org/summarization#Serbian">
        <rdf:type rdf:resource="http://www.example.org/summarization#Non-English"/>
    </owl:NamedIndividual>
    


    <!-- http://www.example.org/summarization#SerbianCyrillic -->

    <owl:NamedIndividual rdf:about="http://www.example.org/summarization#SerbianCyrillic">
        <rdf:type rdf:resource="http://www.example.org/summarization#Non-English"/>
    </owl:NamedIndividual>
    


    <!-- http://www.example.org/summarization#SerbianLatin -->

    <owl:NamedIndividual rdf:about="http://www.example.org/summarization#SerbianLatin">
        <rdf:type rdf:resource="http://www.example.org/summarization#Non-English"/>
    </owl:NamedIndividual>
    


    <!-- http://www.example.org/summarization#ShannonGame -->

    <owl:NamedIndividual rdf:about="http://www.example.org/summarization#ShannonGame">
        <rdf:type rdf:resource="http://www.example.org/summarization#InformationRetrieval"/>
    </owl:NamedIndividual>
    


    <!-- http://www.example.org/summarization#Sinhala -->

    <owl:NamedIndividual rdf:about="http://www.example.org/summarization#Sinhala">
        <rdf:type rdf:resource="http://www.example.org/summarization#Non-English"/>
    </owl:NamedIndividual>
    


    <!-- http://www.example.org/summarization#Slovak -->

    <owl:NamedIndividual rdf:about="http://www.example.org/summarization#Slovak">
        <rdf:type rdf:resource="http://www.example.org/summarization#Non-English"/>
    </owl:NamedIndividual>
    


    <!-- http://www.example.org/summarization#Slovenian -->

    <owl:NamedIndividual rdf:about="http://www.example.org/summarization#Slovenian">
        <rdf:type rdf:resource="http://www.example.org/summarization#Non-English"/>
    </owl:NamedIndividual>
    


    <!-- http://www.example.org/summarization#SogouCA -->

    <owl:NamedIndividual rdf:about="http://www.example.org/summarization#SogouCA">
        <rdf:type rdf:resource="http://www.example.org/summarization#BenchmarkDatasets"/>
        <isAvailableInLanguage rdf:resource="http://www.example.org/summarization#Chinese"/>
    </owl:NamedIndividual>
    


    <!-- http://www.example.org/summarization#Somali -->

    <owl:NamedIndividual rdf:about="http://www.example.org/summarization#Somali">
        <rdf:type rdf:resource="http://www.example.org/summarization#Non-English"/>
    </owl:NamedIndividual>
    


    <!-- http://www.example.org/summarization#Spanish -->

    <owl:NamedIndividual rdf:about="http://www.example.org/summarization#Spanish">
        <rdf:type rdf:resource="http://www.example.org/summarization#Non-English"/>
    </owl:NamedIndividual>
    


    <!-- http://www.example.org/summarization#SumBasic -->

    <owl:NamedIndividual rdf:about="http://www.example.org/summarization#SumBasic">
        <rdfs:comment>An extractive summarization model that implements the SumBasic algorithm, which probabilistically selects sentences for inclusion in the summary based on their individual importance scores derived from word probabilities, favoring sentences containing high-probability words.</rdfs:comment>
        <rdfs:comment>An extractive summarization model that iteratively selects sentences with the highest probability of containing important words.</rdfs:comment>
    </owl:NamedIndividual>
    


    <!-- http://www.example.org/summarization#SumGAN -->

    <owl:NamedIndividual rdf:about="http://www.example.org/summarization#SumGAN">
        <rdfs:comment>An abstractive summarization model that employs Generative Adversarial Networks (GANs) to generate summaries with improved fluency and coherence.</rdfs:comment>
    </owl:NamedIndividual>
    


    <!-- http://www.example.org/summarization#SummBank -->

    <owl:NamedIndividual rdf:about="http://www.example.org/summarization#SummBank">
        <rdf:type rdf:resource="http://www.example.org/summarization#BenchmarkDatasets"/>
        <isAvailableInLanguage rdf:resource="http://www.example.org/summarization#Chinese"/>
        <isAvailableInLanguage rdf:resource="http://www.example.org/summarization#English"/>
        <sourceLink>https://catalog.ldc.upenn.edu/LDC2021T09</sourceLink>
    </owl:NamedIndividual>
    


    <!-- http://www.example.org/summarization#SummEval -->

    <owl:NamedIndividual rdf:about="http://www.example.org/summarization#SummEval">
        <rdf:type rdf:resource="http://www.example.org/summarization#BenchmarkDatasets"/>
        <sourceLink>https://github.com/Yale-LILY/SummEval</sourceLink>
    </owl:NamedIndividual>
    


    <!-- http://www.example.org/summarization#SummScreen -->

    <owl:NamedIndividual rdf:about="http://www.example.org/summarization#SummScreen">
        <rdf:type rdf:resource="http://www.example.org/summarization#BenchmarkDatasets"/>
    </owl:NamedIndividual>
    


    <!-- http://www.example.org/summarization#SummaQA -->

    <owl:NamedIndividual rdf:about="http://www.example.org/summarization#SummaQA">
        <rdf:type rdf:resource="http://www.example.org/summarization#QABased"/>
    </owl:NamedIndividual>
    


    <!-- http://www.example.org/summarization#SummaRuNNer -->

    <owl:NamedIndividual rdf:about="http://www.example.org/summarization#SummaRuNNer">
        <rdfs:comment>An abstractive summarization model that utilizes Recurrent Neural Networks (RNNs) to generate summaries by selecting salient sentences and rewriting them.</rdfs:comment>
    </owl:NamedIndividual>
    


    <!-- http://www.example.org/summarization#Swahili -->

    <owl:NamedIndividual rdf:about="http://www.example.org/summarization#Swahili">
        <rdf:type rdf:resource="http://www.example.org/summarization#Non-English"/>
    </owl:NamedIndividual>
    


    <!-- http://www.example.org/summarization#Swedish -->

    <owl:NamedIndividual rdf:about="http://www.example.org/summarization#Swedish">
        <rdf:type rdf:resource="http://www.example.org/summarization#Non-English"/>
    </owl:NamedIndividual>
    


    <!-- http://www.example.org/summarization#SwissText -->

    <owl:NamedIndividual rdf:about="http://www.example.org/summarization#SwissText">
        <rdf:type rdf:resource="http://www.example.org/summarization#BenchmarkDatasets"/>
        <isAvailableInLanguage rdf:resource="http://www.example.org/summarization#German"/>
    </owl:NamedIndividual>
    


    <!-- http://www.example.org/summarization#T5 -->

    <owl:NamedIndividual rdf:about="http://www.example.org/summarization#T5">
        <rdfs:comment>A versatile abstractive summarization model based on Text-To-Text Transfer Transformer (T5) architecture.</rdfs:comment>
        <rdfs:comment>An abstractive summarization model based on Text-To-Text Transfer Transformer (T5), which formulates summarization as a text-to-text task, enabling it to handle various text generation tasks, including summarization.</rdfs:comment>
    </owl:NamedIndividual>
    


    <!-- http://www.example.org/summarization#TAC -->

    <owl:NamedIndividual rdf:about="http://www.example.org/summarization#TAC">
        <rdf:type rdf:resource="http://www.example.org/summarization#BenchmarkDatasets"/>
        <sourceLink>https://tac.nist.gov/data/index.html</sourceLink>
    </owl:NamedIndividual>
    


    <!-- http://www.example.org/summarization#TAC2008 -->

    <owl:NamedIndividual rdf:about="http://www.example.org/summarization#TAC2008">
        <rdf:type rdf:resource="http://www.example.org/summarization#BenchmarkDatasets"/>
        <sourceLink>https://tac.nist.gov/2008/summarization/</sourceLink>
    </owl:NamedIndividual>
    


    <!-- http://www.example.org/summarization#TAC2009 -->

    <owl:NamedIndividual rdf:about="http://www.example.org/summarization#TAC2009">
        <rdf:type rdf:resource="http://www.example.org/summarization#BenchmarkDatasets"/>
        <sourceLink>https://tac.nist.gov/2009/summarization/</sourceLink>
        <rdfs:label>TAC 2009</rdfs:label>
    </owl:NamedIndividual>
    


    <!-- http://www.example.org/summarization#TAC2010 -->

    <owl:NamedIndividual rdf:about="http://www.example.org/summarization#TAC2010">
        <rdf:type rdf:resource="http://www.example.org/summarization#BenchmarkDatasets"/>
        <rdfs:label>TAC 2010</rdfs:label>
    </owl:NamedIndividual>
    


    <!-- http://www.example.org/summarization#TAC2011 -->

    <owl:NamedIndividual rdf:about="http://www.example.org/summarization#TAC2011">
        <rdf:type rdf:resource="http://www.example.org/summarization#BenchmarkDatasets"/>
        <rdfs:label>TAC 2011</rdfs:label>
    </owl:NamedIndividual>
    


    <!-- http://www.example.org/summarization#TDT -->

    <owl:NamedIndividual rdf:about="http://www.example.org/summarization#TDT">
        <rdf:type rdf:resource="http://www.example.org/summarization#BenchmarkDatasets"/>
        <rdfs:label>Topic Detection and Tracking (TDT)</rdfs:label>
    </owl:NamedIndividual>
    


    <!-- http://www.example.org/summarization#TFIDF -->

    <owl:NamedIndividual rdf:about="http://www.example.org/summarization#TFIDF">
        <rdfs:comment>An extractive summarization model based on the Term Frequency-Inverse Document Frequency (TF-IDF) algorithm, which computes the importance of each word in a document based on its frequency in the document and rarity in the corpus, selecting sentences with high TF-IDF scores for inclusion in the summary.</rdfs:comment>
        <rdfs:comment>An extractive summarization model that selects sentences based on their importance calculated using TF-IDF scores.</rdfs:comment>
    </owl:NamedIndividual>
    


    <!-- http://www.example.org/summarization#TFIDFTextRank -->

    <owl:NamedIndividual rdf:about="http://www.example.org/summarization#TFIDFTextRank">
        <rdfs:comment>An extractive summarization model that combines TF-IDF (Term Frequency-Inverse Document Frequency) and TextRank algorithms to identify and rank important sentences for summarization.</rdfs:comment>
    </owl:NamedIndividual>
    


    <!-- http://www.example.org/summarization#TIPSTER -->

    <owl:NamedIndividual rdf:about="http://www.example.org/summarization#TIPSTER">
        <rdf:type rdf:resource="http://www.example.org/summarization#BenchmarkDatasets"/>
    </owl:NamedIndividual>
    


    <!-- http://www.example.org/summarization#Tamil -->

    <owl:NamedIndividual rdf:about="http://www.example.org/summarization#Tamil">
        <rdf:type rdf:resource="http://www.example.org/summarization#Non-English"/>
    </owl:NamedIndividual>
    


    <!-- http://www.example.org/summarization#TeMrioCorpus -->

    <owl:NamedIndividual rdf:about="http://www.example.org/summarization#TeMrioCorpus">
        <rdf:type rdf:resource="http://www.example.org/summarization#BenchmarkDatasets"/>
        <isAvailableInLanguage rdf:resource="http://www.example.org/summarization#BrazilianPortuguese"/>
    </owl:NamedIndividual>
    


    <!-- http://www.example.org/summarization#Telugu -->

    <owl:NamedIndividual rdf:about="http://www.example.org/summarization#Telugu">
        <rdf:type rdf:resource="http://www.example.org/summarization#Non-English"/>
    </owl:NamedIndividual>
    


    <!-- http://www.example.org/summarization#TextRank -->

    <owl:NamedIndividual rdf:about="http://www.example.org/summarization#TextRank">
        <rdf:type rdf:resource="http://www.example.org/summarization#GraphApproaches"/>
        <rdfs:comment>An extractive summarization model that utilizes the TextRank algorithm, which extends the PageRank algorithm to identify important sentences by treating them as nodes in a graph and computing their importance scores based on the similarity and connections between sentences.</rdfs:comment>
    </owl:NamedIndividual>
    


    <!-- http://www.example.org/summarization#Thai -->

    <owl:NamedIndividual rdf:about="http://www.example.org/summarization#Thai">
        <rdf:type rdf:resource="http://www.example.org/summarization#Non-English"/>
    </owl:NamedIndividual>
    


    <!-- http://www.example.org/summarization#TheEssexArabicSummariesCorpus -->

    <owl:NamedIndividual rdf:about="http://www.example.org/summarization#TheEssexArabicSummariesCorpus">
        <rdf:type rdf:resource="http://www.example.org/summarization#BenchmarkDatasets"/>
    </owl:NamedIndividual>
    


    <!-- http://www.example.org/summarization#TheHindu -->

    <owl:NamedIndividual rdf:about="http://www.example.org/summarization#TheHindu">
        <rdf:type rdf:resource="http://www.example.org/summarization#BenchmarkDatasets"/>
        <isAvailableInLanguage rdf:resource="http://www.example.org/summarization#English"/>
        <isAvailableInLanguage rdf:resource="http://www.example.org/summarization#Hindi"/>
    </owl:NamedIndividual>
    


    <!-- http://www.example.org/summarization#Tigrinya -->

    <owl:NamedIndividual rdf:about="http://www.example.org/summarization#Tigrinya">
        <rdf:type rdf:resource="http://www.example.org/summarization#Non-English"/>
    </owl:NamedIndividual>
    


    <!-- http://www.example.org/summarization#TimesOfIndia -->

    <owl:NamedIndividual rdf:about="http://www.example.org/summarization#TimesOfIndia">
        <rdf:type rdf:resource="http://www.example.org/summarization#BenchmarkDatasets"/>
        <isAvailableInLanguage rdf:resource="http://www.example.org/summarization#Hindi"/>
        <isAvailableInLanguage></isAvailableInLanguage>
    </owl:NamedIndividual>
    


    <!-- http://www.example.org/summarization#Transformer -->

    <owl:NamedIndividual rdf:about="http://www.example.org/summarization#Transformer">
        <rdfs:comment>An abstractive summarization model based on the Transformer architecture, which leverages self-attention mechanisms to capture global dependencies and generate coherent summaries.</rdfs:comment>
    </owl:NamedIndividual>
    


    <!-- http://www.example.org/summarization#Turkish -->

    <owl:NamedIndividual rdf:about="http://www.example.org/summarization#Turkish">
        <rdf:type rdf:resource="http://www.example.org/summarization#Non-English"/>
    </owl:NamedIndividual>
    


    <!-- http://www.example.org/summarization#Twitter -->

    <owl:NamedIndividual rdf:about="http://www.example.org/summarization#Twitter">
        <rdf:type rdf:resource="http://www.example.org/summarization#BenchmarkDatasets"/>
        <isAvailableInLanguage rdf:resource="http://www.example.org/summarization#English"/>
    </owl:NamedIndividual>
    


    <!-- http://www.example.org/summarization#Ukrainian -->

    <owl:NamedIndividual rdf:about="http://www.example.org/summarization#Ukrainian">
        <rdf:type rdf:resource="http://www.example.org/summarization#Non-English"/>
    </owl:NamedIndividual>
    


    <!-- http://www.example.org/summarization#UnifiedSum -->

    <owl:NamedIndividual rdf:about="http://www.example.org/summarization#UnifiedSum">
        <rdf:type rdf:resource="http://www.example.org/summarization#AttentionBased"/>
        <rdfs:comment>An abstractive summarization model that unifies pretraining and fine-tuning approaches to achieve state-of-the-art results across various summarization tasks.</rdfs:comment>
    </owl:NamedIndividual>
    


    <!-- http://www.example.org/summarization#Urdu -->

    <owl:NamedIndividual rdf:about="http://www.example.org/summarization#Urdu">
        <rdf:type rdf:resource="http://www.example.org/summarization#Non-English"/>
    </owl:NamedIndividual>
    


    <!-- http://www.example.org/summarization#Uzbek -->

    <owl:NamedIndividual rdf:about="http://www.example.org/summarization#Uzbek">
        <rdf:type rdf:resource="http://www.example.org/summarization#Non-English"/>
    </owl:NamedIndividual>
    


    <!-- http://www.example.org/summarization#VariationalAutoEncoder -->

    <owl:NamedIndividual rdf:about="http://www.example.org/summarization#VariationalAutoEncoder">
        <rdf:type rdf:resource="http://www.example.org/summarization#NeuralNetworkApproach"/>
    </owl:NamedIndividual>
    


    <!-- http://www.example.org/summarization#Vietnamese -->

    <owl:NamedIndividual rdf:about="http://www.example.org/summarization#Vietnamese">
        <rdf:type rdf:resource="http://www.example.org/summarization#Non-English"/>
    </owl:NamedIndividual>
    


    <!-- http://www.example.org/summarization#WebOfScienceCoreCollection -->

    <owl:NamedIndividual rdf:about="http://www.example.org/summarization#WebOfScienceCoreCollection">
        <rdf:type rdf:resource="http://www.example.org/summarization#BenchmarkDatasets"/>
    </owl:NamedIndividual>
    


    <!-- http://www.example.org/summarization#WebOfScienceCoreCollectionDatabase -->

    <owl:NamedIndividual rdf:about="http://www.example.org/summarization#WebOfScienceCoreCollectionDatabase">
        <rdf:type rdf:resource="http://www.example.org/summarization#BenchmarkDatasets"/>
        <isAvailableInLanguage rdf:resource="http://www.example.org/summarization#English"/>
    </owl:NamedIndividual>
    


    <!-- http://www.example.org/summarization#Weibo -->

    <owl:NamedIndividual rdf:about="http://www.example.org/summarization#Weibo">
        <rdf:type rdf:resource="http://www.example.org/summarization#BenchmarkDatasets"/>
        <isAvailableInLanguage rdf:resource="http://www.example.org/summarization#Chinese"/>
    </owl:NamedIndividual>
    


    <!-- http://www.example.org/summarization#Welsh -->

    <owl:NamedIndividual rdf:about="http://www.example.org/summarization#Welsh">
        <rdf:type rdf:resource="http://www.example.org/summarization#Non-English"/>
    </owl:NamedIndividual>
    


    <!-- http://www.example.org/summarization#Wiki-How -->

    <owl:NamedIndividual rdf:about="http://www.example.org/summarization#Wiki-How">
        <rdf:type rdf:resource="http://www.example.org/summarization#BenchmarkDatasets"/>
    </owl:NamedIndividual>
    


    <!-- http://www.example.org/summarization#WikiCatSum -->

    <owl:NamedIndividual rdf:about="http://www.example.org/summarization#WikiCatSum">
        <rdf:type rdf:resource="http://www.example.org/summarization#BenchmarkDatasets"/>
    </owl:NamedIndividual>
    


    <!-- http://www.example.org/summarization#WikiLingua -->

    <owl:NamedIndividual rdf:about="http://www.example.org/summarization#WikiLingua">
        <rdf:type rdf:resource="http://www.example.org/summarization#BenchmarkDatasets"/>
    </owl:NamedIndividual>
    


    <!-- http://www.example.org/summarization#Wikipedia -->

    <owl:NamedIndividual rdf:about="http://www.example.org/summarization#Wikipedia">
        <rdf:type rdf:resource="http://www.example.org/summarization#BenchmarkDatasets"/>
        <isAvailableInLanguage rdf:resource="http://www.example.org/summarization#English"/>
    </owl:NamedIndividual>
    


    <!-- http://www.example.org/summarization#XL-Sum -->

    <owl:NamedIndividual rdf:about="http://www.example.org/summarization#XL-Sum">
        <rdf:type rdf:resource="http://www.example.org/summarization#BenchmarkDatasets"/>
        <isAvailableInLanguage rdf:resource="http://www.example.org/summarization#Amharic"/>
        <isAvailableInLanguage rdf:resource="http://www.example.org/summarization#Korean"/>
        <isAvailableInLanguage rdf:resource="http://www.example.org/summarization#Yoruba"/>
    </owl:NamedIndividual>
    


    <!-- http://www.example.org/summarization#XLNet -->

    <owl:NamedIndividual rdf:about="http://www.example.org/summarization#XLNet">
        <rdfs:comment>A powerful abstractive summarization model based on XLNet, a generalized autoregressive pretraining method.</rdfs:comment>
    </owl:NamedIndividual>
    


    <!-- http://www.example.org/summarization#XLSum -->

    <owl:NamedIndividual rdf:about="http://www.example.org/summarization#XLSum">
        <rdf:type rdf:resource="http://www.example.org/summarization#BenchmarkDatasets"/>
        <sourceLink>https://github.com/csebuetnlp/xl-sum</sourceLink>
    </owl:NamedIndividual>
    


    <!-- http://www.example.org/summarization#XSum -->

    <owl:NamedIndividual rdf:about="http://www.example.org/summarization#XSum">
        <rdf:type rdf:resource="http://www.example.org/summarization#BenchmarkDatasets"/>
        <isAvailableInLanguage rdf:resource="http://www.example.org/summarization#English"/>
        <isAvailableInLanguage rdf:resource="http://www.example.org/summarization#Korean"/>
    </owl:NamedIndividual>
    


    <!-- http://www.example.org/summarization#Yoruba -->

    <owl:NamedIndividual rdf:about="http://www.example.org/summarization#Yoruba">
        <rdf:type rdf:resource="http://www.example.org/summarization#Non-English"/>
    </owl:NamedIndividual>
    


    <!-- http://www.example.org/summarization#ebay -->

    <owl:NamedIndividual rdf:about="http://www.example.org/summarization#ebay">
        <rdf:type rdf:resource="http://www.example.org/summarization#BenchmarkDatasets"/>
    </owl:NamedIndividual>
    


    <!-- http://www.example.org/summarization#iSTS -->

    <owl:NamedIndividual rdf:about="http://www.example.org/summarization#iSTS">
        <rdf:type rdf:resource="http://www.example.org/summarization#SimilarityBased"/>
    </owl:NamedIndividual>

    <owl:NamedIndividual rdf:about="http://www.example.org/summarization#BERTSum">
    <rdfs:comment>A summarization model utilizing BERT's language understanding capabilities for extractive summarization.</rdfs:comment>
</owl:NamedIndividual>

<owl:NamedIndividual rdf:about="http://www.example.org/summarization#GPT2Sum">
    <rdfs:comment>An abstractive summarization model leveraging GPT-2's generative abilities to create concise summaries.</rdfs:comment>
</owl:NamedIndividual>

<owl:NamedIndividual rdf:about="http://www.example.org/summarization#PointerGenerator">
    <rdfs:comment>A hybrid model combining extractive and abstractive techniques, using a pointer-generator network for summarization.</rdfs:comment>
</owl:NamedIndividual>

<owl:NamedIndividual rdf:about="http://www.example.org/summarization#T5Sum">
    <rdfs:comment>Utilizes the Text-to-Text Transfer Transformer (T5) for abstractive summarization, generating summaries by rephrasing content.</rdfs:comment>
</owl:NamedIndividual>

<owl:NamedIndividual rdf:about="http://www.example.org/summarization#XLNetSum">
    <rdfs:comment>An advanced model based on XLNet for abstractive text summarization, enhancing context understanding in summaries.</rdfs:comment>
</owl:NamedIndividual>

<owl:NamedIndividual rdf:about="http://www.example.org/summarization#Lead3">
    <rdfs:comment>An extractive summarization model that selects the first three sentences of a document as its summary, based on the lead paragraph concept.</rdfs:comment>
</owl:NamedIndividual>

<owl:NamedIndividual rdf:about="http://www.example.org/summarization#LexRank">
    <rdfs:comment>A graph-based extractive summarization model that ranks sentences in a document based on their semantic similarity to produce a summary.</rdfs:comment>
</owl:NamedIndividual>

<owl:NamedIndividual rdf:about="http://www.example.org/summarization#LuhnSum">
    <rdfs:comment>Utilizes Luhn's heuristic method for extractive summarization, emphasizing the significance of high-frequency words in generating summaries.</rdfs:comment>
</owl:NamedIndividual>

<owl:NamedIndividual rdf:about="http://www.example.org/summarization#TextRank">
    <rdfs:comment>A graph-based, extractive summarization model that leverages the TextRank algorithm to identify key sentences for summary generation.</rdfs:comment>
</owl:NamedIndividual>

<owl:NamedIndividual rdf:about="http://www.example.org/summarization#NeuralAttention">
    <rdfs:comment>A model employing neural attention mechanisms to focus on key parts of the text for abstractive summarization.</rdfs:comment>
</owl:NamedIndividual>

<owl:NamedIndividual rdf:about="http://www.example.org/summarization#OpenNMTSum">
    <rdfs:comment>Based on the OpenNMT toolkit, this model applies neural machine translation techniques for abstractive text summarization.</rdfs:comment>
</owl:NamedIndividual>

<owl:NamedIndividual rdf:about="http://www.example.org/summarization#SummaRuNNer">
    <rdfs:comment>An extractive summarization model that uses a recurrent neural network to rank sentences for inclusion in the summary.</rdfs:comment>
</owl:NamedIndividual>

<owl:NamedIndividual rdf:about="http://www.example.org/summarization#TransformerSum">
    <rdfs:comment>Utilizes the Transformer architecture for abstractive summarization, focusing on improving the generation of coherent and concise summaries.</rdfs:comment>
</owl:NamedIndividual>


<!-- Abstractive Individuals -->
<owl:NamedIndividual rdf:about="http://www.co-ode.org/ontologies/ont.owl#BanditSum">
    <rdfs:comment>A model that optimizes sentence selection for summaries using reinforcement learning techniques to achieve better coherence and relevance.</rdfs:comment>
</owl:NamedIndividual>

<owl:NamedIndividual rdf:about="http://www.co-ode.org/ontologies/ont.owl#Seq2Seq">
    <rdfs:comment>A framework employing encoder-decoder architectures to generate summaries by understanding and rephrasing the original text.</rdfs:comment>
</owl:NamedIndividual>

<!-- Extractive Individuals -->
<owl:NamedIndividual rdf:about="http://www.example.org/summarization#AbsN">
    <rdfs:comment>Selects sentences for summarization based on their absolute length, assuming longer sentences convey more value.</rdfs:comment>
</owl:NamedIndividual>

<owl:NamedIndividual rdf:about="http://www.example.org/summarization#GraphApproaches">
    <rdfs:comment>Implements graph-based models, such as TextRank, to identify and extract the most relevant sentences based on the document's semantic structure.</rdfs:comment>
</owl:NamedIndividual>

<owl:NamedIndividual rdf:about="http://www.example.org/summarization#LengthBased">
    <rdfs:comment>Prioritizes sentence selection for summarization strictly based on their length, under the assumption that longer sentences provide more informational value.</rdfs:comment>
</owl:NamedIndividual>

<!-- Hybrid Individuals -->
<owl:NamedIndividual rdf:about="http://www.example.org/summarization#AttentionBased">
    <rdfs:comment>Leverages attention mechanisms to focus on significant parts of the text, combining extractive and abstractive methods for summarization.</rdfs:comment>
</owl:NamedIndividual>

<owl:NamedIndividual rdf:about="http://www.example.org/summarization#PointerGeneratorNetworksHybrid">
    <rdfs:comment>A hybrid model combining the benefits of both extractive and abstractive summarization by using a pointer-generator network.</rdfs:comment>
</owl:NamedIndividual>

<owl:NamedIndividual rdf:about="http://www.example.org/summarization#TransformerBasedModelsHybrid">
    <rdfs:comment>Utilizes Transformer architectures to effectively blend extractive and abstractive summarization strategies for comprehensive summaries.</rdfs:comment>
</owl:NamedIndividual>

</rdf:RDF>



<!-- Generated by the OWL API (version 4.5.26.2023-07-17T20:34:13Z) https://github.com/owlcs/owlapi -->
